tacs
git-svn-id: svn://scm.gforge.inria.fr/svn/cfml@280 ba02c806-7d2b-4818-9a48-35b22e6bdc79

imper/Facto_proof.v
@@ -1,5 +1,145 @@
 Set Implicit Arguments.
+
+Require Import LibTactics List.
+
+Ltac forwards_nounfold_then Ei cont ::=
+  let args := ltac_args Ei in
+  let args := (eval simpl in (args ++ ((boxer ___)::nil))) in
+  build_app args cont;
+  fast_rm_inside Ei.
+
 Require Import CFLib Facto_ml.
+
+Notation "'While' Q1 'Do' Q2 '_Done'" :=
+  (!While (fun H Q => forall R:~~unit, is_local R ->
+        (forall H Q, (If_ Q1 Then (Q2 ;; R) Else (Ret tt)) H Q -> R H Q)
+        -> R H Q))
+  (at level 69, Q2 at level 68, only parsing) : charac.
+
+Lemma while_loop_cf_to_inv : 
+   forall (A:Type) (I:A->hprop) (J:A->bool->hprop) (lt:binary A),
+   forall (F1:~~bool) (F2:~~unit) H (Q:unit->hprop),
+   wf lt -> 
+   (exists X0, H ==> (I X0)) ->
+   (forall X, F1 (I X) (J X)
+              /\ F2 (J X true) (# Hexists Y, (I Y) \* [lt Y X])
+              /\ J X false ==> Q tt) ->
+  (While F1 Do F2 _Done) H Q.
+Proof.
+  introv W (X0&I0) M. apply local_erase.
+  introv LR HR. applys* local_weaken (rm I0). gen X0. 
+  intros X. induction_wf IH: W X.
+  destruct (M X) as (M1&M2&M3).
+  applys HR. xlet*. xif. xseq*. xextract as Y L.
+  xapply_local* IH; hsimpl.
+  xret. destruct x; auto_false.
+Qed.
+
+
+Notation "'For' i '=' a 'To' b 'Do' Q1 '_Done'" :=
+  (!For (fun H Q => forall S:int->~~unit, is_local_1 S ->
+        (forall i H Q,  
+             (i <= (b)%Z -> (Q1 ;; S (i+1)) H Q)
+          /\ (i > b%Z -> (Ret tt) H Q) 
+          -> S i H Q)
+       -> S a H Q))
+  (at level 69, i ident, a at level 0, b at level 0) : charac.
+
+
+Lemma for_loop_cf_to_inv : 
+   forall I H',
+   forall (a:int) (b:int) (F:~~unit) H (Q:unit->hprop),
+   (a > (b)%Z -> H ==> (Q tt)) ->
+   (a <= (b)%Z ->
+          (H ==> I a \* H') 
+       /\ (forall i, a <= i /\ i <= (b)%Z -> F (I i) (# I(i+1))) 
+       /\ (I ((b)%Z+1) \* H' ==> Q tt)) ->
+  (For i = a To b Do F _Done) H Q.
+Proof.
+  introv M1 M2. apply local_erase. intros S LS HS.
+  tests (a > b) as C. 
+  apply (rm HS). split; intros C'. math. xret~.
+  forwards (Ma&Mb&Mc): (rm M2). math.
+   cuts P: (forall i, a <= i <= b+1 -> S i (I i) (# I (b+1))).
+     xapply_local P. math. hchanges Ma. hchanges Mc.
+   intros i. induction_wf IH: (int_upto_wf (b+1)) i. intros Bnd.
+   applys (rm HS). split; intros C'.
+     xseq. eapply Mb. math. xapply_local IH; auto with maths; hsimpl.
+  xret. math_rewrite~ (i = b +1).  
+Qed.
+
+
+
+(********************************************************************)
+(* ** Loop invariants for while-loops *)
+
+Definition while_loop_cf (F1:~~bool) (F2:~~unit) :=
+  local (fun (H:hprop) (Q:unit->hprop) => forall R:~~unit, is_local R ->
+    (forall H Q, (exists Q', F1 H Q' 
+       /\ (local (fun H Q => exists Q', F2 H Q' /\ R (Q' tt) Q) (Q' true) Q)
+       /\ Q' false ==> Q tt) -> R H Q) 
+    -> R H Q).
+
+Definition while_loop_inv (F1:~~bool) (F2:~~unit) :=
+  local (fun (H:hprop) (Q:unit->hprop) => 
+    exists A:Type, exists I:A->hprop, exists J:A->bool->hprop, exists lt:binary A,
+      wf lt 
+   /\ (exists X0, H ==> (I X0))
+   /\ (forall X, F1 (I X) (J X)
+              /\ F2 (J X true) (# Hexists Y, (I Y) \* [lt Y X])
+              /\ J X false ==> Q tt)).
+
+Lemma while_loop_cf_to_inv : forall (F1:~~bool) (F2:~~unit),
+  while_loop_inv F1 F2 ===> while_loop_cf F1 F2.
+Proof. 
+  intros. apply local_weaken_body. intros H Q (A&I&J&lt&W&(X0&I0)&M).
+  introv LR HR. applys* local_weaken I0. clear I0. gen X0. 
+  intros X. induction_wf IH: W X.
+  destruct (M X) as (M1&M2&M3).
+  applys HR. exists (J X). splits~.
+  apply local_erase. esplit. split. apply M2. 
+  apply~ local_extract_exists. intros x.
+   rewrite star_comm. apply~ CFHeaps.local_intro_prop'.
+Qed. 
+
+
+(********************************************************************)
+(* ** Loop invariants for for-loops *)
+
+Definition for_loop_cf (a:int) (b:int) (F:~~unit) :=
+  local (fun (H:hprop) (Q:unit->hprop) => forall S:int->~~unit, is_local_1 S ->
+     (forall i H Q,  
+          ((i <= (b)%Z -> (local (fun H Q => exists Q', F H Q' /\ S (i+1) (Q' tt) Q) H Q))
+       /\ (i > b%Z -> H ==> Q tt)) 
+       -> S i H Q)
+    -> S a H Q).
+
+Definition for_loop_inv (a:int) (b:int) (F:~~unit) :=
+  local (fun (H:hprop) (Q:unit->hprop) => 
+      (a > (b)%Z -> H ==> (Q tt)) 
+   /\ (a <= (b)%Z -> exists H', exists I,
+          (H ==> I a \* H') 
+       /\ (forall i, a <= i /\ i <= (b)%Z -> F (I i) (# I(i+1))) 
+       /\ (I ((b)%Z+1) \* H' ==> Q tt))).
+
+Lemma for_loop_cf_to_inv : forall (a:int) (b:int) (F:~~unit),
+  for_loop_inv a b F ===> for_loop_cf a b F.
+Proof. 
+  intros. apply local_weaken_body. intros H Q (Mgt&Mle). introv LS HS.
+  tests (a > b) as C. apply HS. split. math. auto.
+  clear Mgt. specializes Mle. math. destruct Mle as (H'&I&M1&M2&M3).
+  applys~ (@local_wframe unit) (# I (b+1)); [| intros u; destruct~ u ]. 
+  clear M1. asserts L: (a <= a <= b+1). math. generalize L.
+  set (a' := a) at 1. generalize a as i. unfold a'.
+  intros i. induction_wf IH: (int_upto_wf (b+1)) i. intros Bnd.
+  applys HS. split; intros C'.
+    apply local_erase. esplit. split.
+      apply M2; auto with maths.
+      forwards: IH (i+1); auto with maths.
+    math_rewrite~ (i = b +1).
+Qed. 
+
+
 
 Ltac auto_tilde ::= auto with maths.
 
@@ -22,9 +162,9 @@ Lemma facto_rec_spec : Spec facto_rec n |R>>
   n >= 0 -> R [] (\= fact n).
 Proof.
   apply (spec_induction_1_noheap (lt:=downto 0)). prove_wf.
-  xcf. intros. xif. xret.
-  xif_after. xret. xsimpl. rewrite~ fact_zero.
-  xif_after. xapp~. intro_subst. xret. hsimpl. rewrite~ <- fact_succ.
+  xcf. intros. xif.
+  xret. xsimpl. rewrite~ fact_zero.
+  xapp~. intro_subst. xret. hsimpl. rewrite~ <- fact_succ.
 Qed.
 
 
@@ -42,7 +182,7 @@ Proof.
     xseq. xapps. xapp. xapply_local~ IH. 
     hsimpl. math_rewrite (i+1-1 = i). rewrite~ (@fact_succ i). ring.
     hsimpl. xret. hsimpl. fequals. math.
-  xapp. hsimpl.
+  xapp. hsimpl~.
 Qed.
 
 
@@ -52,9 +192,13 @@ Qed.
 Lemma facto_while_spec : Spec facto_while n |R>>
   n >= 0 -> R [] (\= fact n).
 Proof.
-  xcf. intros. xapp. xapp. xwhile.  
+  xcf. intros. xapp. xapp. 
+xuntag. apply while_loop_cf_to_inv.
+
+ xwhile.  
   xgeneralize (forall i:int, R ([0 <= i <= n] \* m ~~> (i+1) \* r ~~> (fact i)) 
-                                              (# m ~~> (n+1) \* r ~~> (fact n))).
+              
+                                (# m ~~> (n+1) \* r ~~> (fact n))).
     xapply_local~ (Inv 0). hsimpl. rewrite~ fact_zero. math.
     intros i. induction_wf IH: (int_upto_wf (n+1)) i. xextract as Gt.
     apply HR. clear HR. xif. xapps. xret.
